added instruction cache flush to model

basetypesScript.sml
@@ -158,16 +158,22 @@ val wt_CA_lem = store_thm("wt_CA_lem", ``
 
 (* core requests to memory *)
 
-val _ = Datatype `corereq = DREQ dop | FREQ padr | NOREQ`;
+val _ = Datatype `corereq = DREQ dop | FREQ padr | ICFR padr | NOREQ`;
 
 val Adr_def = Define `
    (Adr (DREQ dop) = PA dop)
 /\ (Adr (FREQ pa) = pa)
+/\ (Adr (ICFR pa) = pa)
 `;
 
 val Freq_def = Define `
    (Freq (FREQ pa) = T)
 /\ (Freq _ = F)
+`;
+
+val Ireq_def = Define `
+   (Ireq (ICFR pa) = T)
+/\ (Ireq _ = F)
 `;
 
 val Dreq_def = Define `
@@ -192,18 +198,20 @@ val Creq_def = Define `
 
 val CAreq_def = Define `
    (CAreq (DREQ dop) = CA dop)
-/\ (CAreq (FREQ pa) = T)
 /\ (CAreq NOREQ = F)
+/\ (CAreq _ = T)
 `;
 
 val Acc_def = Define `
    (Acc (DREQ dop) = if wt dop then W else R)
 /\ (Acc (FREQ pa) = EX)
+/\ (Acc (ICFR pa) = R)
 `;
 
 val Dop_def = Define `
    (Dop (DREQ dop) = dop)
 /\ (Dop (FREQ pa) = RD pa T)
+/\ (Dop (ICFR pa) = CL pa)
 `;
 
 val Freq_lem = store_thm("Freq_lem", ``
@@ -211,6 +219,14 @@ val Freq_lem = store_thm("Freq_lem", ``
 ``,
   Cases >> (
       RW_TAC std_ss [Freq_def]
+  )
+);
+
+val Ireq_lem = store_thm("Ireq_lem", ``
+!req. Ireq req ==> ?pa. req = ICFR pa
+``,
+  Cases >> (
+      RW_TAC std_ss [Ireq_def]
   )
 );
 
@@ -247,21 +263,23 @@ val Creq_lem = store_thm("Creq_lem", ``
 );
 
 val not_Wreq_lem = store_thm("not_Wreq_lem", ``
-!req. (Freq req \/ Rreq req \/ Creq req \/ (req = NOREQ)) ==> ~Wreq req
+!req. (Freq req \/ Ireq req \/ Rreq req \/ Creq req \/ (req = NOREQ)) ==>
+    ~Wreq req
 ``,
   Cases >> (
-      RW_TAC std_ss [Freq_def, Rreq_def, Wreq_def, Creq_def] >>
+      RW_TAC std_ss [Freq_def, Ireq_def, Rreq_def, Wreq_def, Creq_def] >>
       METIS_TAC [dop_cases_lem2]
   )
 );
 
 val req_cases_lem = store_thm("req_cases_lem", ``
-!req. Freq req /\ ~Dreq req /\ req <> NOREQ
-   \/ ~Freq req /\ Dreq req /\ req <> NOREQ
-   \/ ~Freq req /\ ~Dreq req /\ (req = NOREQ)
+!req. Freq req /\ ~Ireq req /\ ~Dreq req /\ req <> NOREQ
+   \/ ~Freq req /\ Ireq req /\ ~Dreq req /\ req <> NOREQ
+   \/ ~Freq req /\ ~Ireq req /\ Dreq req /\ req <> NOREQ
+   \/ ~Freq req /\ ~Ireq req /\ ~Dreq req /\ (req = NOREQ)
 ``,
   Cases >> (
-      RW_TAC std_ss [Freq_def, Dreq_def]
+      RW_TAC std_ss [Freq_def, Ireq_def, Dreq_def]
   )
 );
 
@@ -278,40 +296,47 @@ val Dreq_cases_lem = store_thm("Dreq_cases_lem", ``
 );
 
 val not_NOREQ_lem = store_thm("not_NOREQ_lem", ``
-!req. req <> NOREQ ==> Dreq req \/ Freq req
+!req. req <> NOREQ ==> Dreq req \/ Freq req \/ Ireq req
 ``,
   METIS_TAC [req_cases_lem]
 );
 
-(* dop list *)
+(* op list *)
 
-val adrs_def = Define `adrs dl = set (MAP PA dl)`;
+val _ = Datatype `mop = DOP dop | IFL padr`;
+
+val opd_def = Define `
+    (opd (DOP dop) = dop)
+ /\ (opd (IFL pa) = CL pa)
+`;
+
+val adrs_def = Define `adrs dl = set (MAP PA (MAP opd dl))`;
 
 val adrs_lem = store_thm("adrs_lem", ``
-!d pa. pa NOTIN adrs [d] ==>  pa <> PA d
+!d pa. pa NOTIN adrs [d] ==>  pa <> PA (opd d)
 ``,
   RW_TAC std_ss [adrs_def] >>
   FULL_SIMP_TAC std_ss [listTheory.MEM_MAP] >>
   FULL_SIMP_TAC std_ss [GSYM IMP_DISJ_THM] >>
   CCONTR_TAC >>
   PAT_X_ASSUM ``!y. x`` (
-      fn thm => ASSUME_TAC ( SPEC ``d:dop`` thm )
+      fn thm => ASSUME_TAC ( SPEC ``opd d`` thm )
   ) >>
   FULL_SIMP_TAC std_ss [listTheory.MEM] 
 );
 
 val adrs_lem2 = store_thm("adrs_lem2", ``
-!d pa. pa IN adrs [d] ==>  (pa = PA d)
+!d pa. pa IN adrs [d] ==>  (pa = PA (opd d))
 ``,
   RW_TAC std_ss [adrs_def] >>
   FULL_SIMP_TAC std_ss [listTheory.MEM_MAP] >>
   FULL_SIMP_TAC std_ss [listTheory.MEM] 
 );
 
-val writes_def = Define `writes dl = set (MAP PA (FILTER wt dl))`;
+val writes_def = Define `writes dl = set (MAP PA (FILTER wt (MAP opd dl)))`;
 
 val writes_lem = store_thm("writes_lem", ``
-!d pa. pa NOTIN writes [d] ==>  ~(wt d /\ (PA d = pa))
+!d pa. pa NOTIN writes [d] ==>  ~(wt (opd d) /\ (PA (opd d) = pa))
 ``,
   RW_TAC std_ss [writes_def] >>
   FULL_SIMP_TAC std_ss [listTheory.MEM_MAP] >>
@@ -319,13 +344,13 @@ val writes_lem = store_thm("writes_lem", ``
   CCONTR_TAC >>
   FULL_SIMP_TAC std_ss [GSYM IMP_DISJ_THM] >>
   PAT_X_ASSUM ``!y. x`` (
-      fn thm => ASSUME_TAC ( SPEC ``d:dop`` thm )
+      fn thm => ASSUME_TAC ( SPEC ``opd d`` thm )
   ) >>
-  FULL_SIMP_TAC std_ss [listTheory.MEM] 
+  REV_FULL_SIMP_TAC std_ss [listTheory.MEM, listTheory.MEM_MAP] 
 );
 
 val writes_lem2 = store_thm("writes_lem2", ``
-!d pa. pa IN writes [d] ==>  wt d /\ (PA d = pa)
+!d pa. pa IN writes [d] ==>  wt (opd d) /\ (PA (opd d) = pa)
 ``,
   RW_TAC std_ss [writes_def] >> (
       FULL_SIMP_TAC std_ss [listTheory.MEM_MAP,
@@ -334,16 +359,17 @@ val writes_lem2 = store_thm("writes_lem2", ``
   )
 );
 
-val reads_def = Define `reads dl = set (MAP PA (FILTER rd dl))`;
+val reads_def = Define `reads dl = set (MAP PA (FILTER rd (MAP opd dl)))`;
 
 val reads_lem = store_thm("reads_lem", ``
-!d pa. pa IN reads [d] ==>  rd d /\ (PA d = pa)
+!d pa. pa IN reads [d] ==>  rd (opd d) /\ (PA (opd d) = pa)
 ``,
   REPEAT GEN_TAC >>
   STRIP_TAC >>
   FULL_SIMP_TAC std_ss [reads_def] >>
   FULL_SIMP_TAC std_ss [listTheory.MEM_MAP] >>
   FULL_SIMP_TAC std_ss [listTheory.MEM_FILTER] >>
+  FULL_SIMP_TAC std_ss [listTheory.MEM_MAP] >>
   IMP_RES_TAC rd_lem >>
   FULL_SIMP_TAC std_ss [listTheory.MEM] 
 );
@@ -353,8 +379,11 @@ val adrs_writes_lem = store_thm("adrs_writes_lem", ``
 ``,
   RW_TAC std_ss [adrs_def, writes_def, listTheory.MEM_MAP] >>
   FULL_SIMP_TAC std_ss [listTheory.MEM_FILTER] >>
-  HINT_EXISTS_TAC >> 
-  ASM_REWRITE_TAC []
+  FULL_SIMP_TAC std_ss [listTheory.MEM_MAP] >>
+  EXISTS_TAC ``y:dop`` >> 
+  ASM_REWRITE_TAC [] >>
+  HINT_EXISTS_TAC  >>
+  ASM_REWRITE_TAC [] 
 );
 
 val not_adrs_not_writes_lem = save_thm("not_adrs_not_writes_lem", 
@@ -363,7 +392,20 @@ adrs_writes_lem |> SPEC_ALL |> CONTRAPOS |> GEN_ALL)
 
 val dops_def = Define `dops dl = set dl`;
 
-val cleans_def = Define `cleans dl = set (MAP PA (FILTER cl dl))`;
+val ifl_def = Define `
+    (ifl (IFL pa) = T)
+ /\ (ifl _ = F)
+`;
+
+val cleans_def = Define `cleans dl = 
+    set (MAP PA (FILTER cl (MAP opd dl)))
+`;
+val icleans_def = Define `icleans dl = 
+    set (MAP PA (MAP opd ((FILTER ifl dl))))
+`;
+val dcleans_def = Define `dcleans dl = 
+    set (MAP PA (FILTER cl (MAP opd (FILTER ($~ o ifl) dl))))
+`;
 
 val not_writes_lem = store_thm("not_writes_lem", ``
 !dl pa. pa IN adrs dl /\ pa NOTIN writes dl ==> 
@@ -371,23 +413,46 @@ val not_writes_lem = store_thm("not_writes_lem", ``
 ``,
   RW_TAC std_ss [adrs_def, writes_def, reads_def, cleans_def, 
 		 listTheory.MEM_MAP] >>
-  Cases_on `y`
-  >| [(* read *)
-      DISJ1_TAC >>
-      EXISTS_TAC ``RD p b`` >>
-      RW_TAC std_ss [listTheory.MEM_FILTER, rd_def]
+  Cases_on `y'`
+  >| [(* DOP *)
+      Cases_on `d`
+      >| [(* read *)
+          DISJ1_TAC >>
+          EXISTS_TAC ``RD p b`` >>
+          RW_TAC std_ss [listTheory.MEM_FILTER, rd_def, opd_def,
+			 listTheory.MEM_MAP] >>
+	  HINT_EXISTS_TAC >>
+	  ASM_REWRITE_TAC [opd_def]
+          ,
+          (* write *)
+          PAT_X_ASSUM ``!y. x`` (
+              fn thm => ASSUME_TAC ( SPEC ``WT p c b`` thm )
+          ) >>
+          FULL_SIMP_TAC std_ss [listTheory.MEM_FILTER, wt_def, opd_def] >>
+	  FULL_SIMP_TAC std_ss [listTheory.MEM_MAP] >>
+          PAT_X_ASSUM ``!y. x`` (
+              fn thm => ASSUME_TAC ( SPEC ``DOP (WT p c b)`` thm )
+          ) >>
+	  FULL_SIMP_TAC std_ss [opd_def]
+          ,
+          (* clean *)
+          DISJ2_TAC >>
+          EXISTS_TAC ``CL p`` >>
+          RW_TAC std_ss [listTheory.MEM_FILTER, cl_def, opd_def,
+			 listTheory.MEM_MAP] >>
+	  HINT_EXISTS_TAC >>
+	  ASM_REWRITE_TAC [opd_def]
+         ]
       ,
-      (* clean *)
-      PAT_X_ASSUM ``!y. x`` (
-          fn thm => ASSUME_TAC ( SPEC ``WT p c b`` thm )
-      ) >>
-      FULL_SIMP_TAC std_ss [listTheory.MEM_FILTER, wt_def]
-      ,
-      (* clean *)
+      (* IFL *)
+      FULL_SIMP_TAC std_ss [opd_def] >>
       DISJ2_TAC >>
-      EXISTS_TAC ``CL p`` >>
-      RW_TAC std_ss [listTheory.MEM_FILTER, cl_def]
-     ]      
+      EXISTS_TAC ``CL p``>>
+      ASM_REWRITE_TAC [listTheory.MEM_FILTER] >>
+      ASM_REWRITE_TAC [cl_def, listTheory.MEM_MAP] >>
+      HINT_EXISTS_TAC >>
+      ASM_REWRITE_TAC [opd_def]
+     ]
 );
 
 (*********** finish ************)
